BetreeSpecCommon / BetreeSpec

disk-betree/BlockInterface.dfy
@@ -67,6 +67,11 @@ abstract module BlockInterface refines Transactable {
     && s'.view == s.view[ref := block]
   }
 
+  predicate Reads(k: Constants, s: Variables, ref: Reference, block: Node)
+  {
+    IMapsTo(s.view, ref, block)
+  }
+
   predicate OpStep(k: Constants, s: Variables, s': Variables, op: Op)
   {
     match op {
